moving from local logs in AE to a single global log. WIP

secure_api/box/Box.AE.fst
@@ -7,8 +7,8 @@
 module Box.AE
 
 open FStar.Set
-open FStar.HyperStack
 open FStar.HyperHeap
+open FStar.HyperStack
 open FStar.Monotonic.RRef
 open FStar.Endianness
 
@@ -19,6 +19,7 @@ open Box.Indexing
 
 module MR = FStar.Monotonic.RRef
 module HH = FStar.HyperHeap
+module HS = FStar.HyperStack
 module MM = MonotoneMap
 module SPEC = Spec.SecretBox
 
@@ -37,48 +38,32 @@ val create_zero_bytes: n:nat -> Tot (b:bytes{Seq.length b = n})
 let create_zero_bytes n =
   Seq.create n (UInt8.uint_to_t 0)
 
-assume val ae_key_region: (r:MR.rid{ extends r root 
+
+assume val ae_log_region: (r:MR.rid{ extends r root 
 				     /\ is_eternal_region r 
 				     /\ is_below r root
 				     /\ disjoint r id_log_region
 				     /\ disjoint r id_honesty_log_region
 				     })
 
-type log_key = nonce
-type log_value (i:id{AE_id? i}) = (cipher*protected_ae_plain i)
-type log_range = fun (i:id{AE_id? i}) -> (fun log_key -> (log_value i))
-type log_inv (i:id{AE_id? i}) (f:MM.map' log_key (log_range i)) = True
+type ae_log_key = (nonce*(i:id{AE_id? i}))
+type ae_log_value (i:id{AE_id? i}) = (cipher*protected_ae_plain i)
+type ae_log_range = fun (k:ae_log_key) -> ae_log_value (snd k)
+type ae_log_inv (f:MM.map' ae_log_key ae_log_range) = True
 
-(**
-   log_t is a monotone map that maps nonces to a tuple of ciphertext and plaintext. It is instantiated in the key type
-   to provide the following guarantee in case the key is honest and AE is idealized:
-   * Authentication: Upon encryption, the message is stored in the log, indexed by the nonce. Upon decryption, a lookup
-     is performed using the nonce received and if the ciphertext in the log matches the received ciphertext, the plaintext
-     is extracted from the log.
-   The log will give the following guarantee regardless of the honesty of the key or the idealization of AE:
-   * Nonce uniqueness: Every log can only have one entry per index. Since the nonce is used as the index in the log, a nonce
-     can only be used once per key.
-   
-*)
-type log_t (i:id{AE_id? i}) (r:rid)  = MM.t r log_key (log_range i) (log_inv i)
 
-(**
-   empty_log returns an empty monotone map of type log_t. 
-*)
-val empty_log: i:id{AE_id? i} -> Tot (MM.map' log_key (log_range i))
-let empty_log i = MM.empty_map log_key (log_range i)
+assume val ae_log: MM.t ae_log_region ae_log_key ae_log_range ae_log_inv
 
 (**
    The key type is abstract and can only be accessed via the leak and coerce_key functions. This means that the adversary has no means
    of accessing the raw representation of any honest AE key if AE is idealized.
 *)
 noeq abstract type key =
-  | Key: #i:id{AE_id? i /\ unfresh i /\ registered i} -> #(region:rid{extends region ae_key_region /\ is_below region ae_key_region /\ is_eternal_region region}) -> raw:aes_key -> log:log_t i region -> key
+  | Key: #i:id{AE_id? i /\ unfresh i /\ registered i} -> raw:aes_key -> key
 
 val get_index: k:key -> Tot (i:id{i=k.i /\ AE_id? i})
 let get_index k = k.i
 
-#set-options "--z3rlimit 25"
 (**
    This function generates a fresh random key. Honest, as well as dishonest ids can be created using keygen. However, note that the adversary can
    only access the raw representation of dishonest keys. The log is created in a fresh region below the ae_key_region.
@@ -89,23 +74,15 @@ val keygen: i:id{AE_id? i} -> ST (k:key{k.i=i})
     /\ registered i // We require this to enforce a static corruption model.
   ))
   (ensures  (fun h0 k h1 -> 
-    let (s:Set.set (HH.rid)) = Set.union (Set.singleton k.region) (Set.singleton id_log_region) in
+    let (s:Set.set (HH.rid)) = Set.singleton id_log_region in
     HH.modifies_just s h0.h h1.h
-    /\ extends k.region ae_key_region
-    /\ fresh_region k.region h0.h h1.h
-    /\ is_below k.region ae_key_region
-    /\ m_contains k.log h1
-    /\ m_sel h1 k.log == MM.empty_map log_key (log_range k.i)
     /\ makes_unfresh_just i h0 h1
   ))
 let keygen i =
   MR.m_recall id_log;
   make_unfresh i;
   let rnd_k = random_bytes (UInt32.uint_to_t keysize) in
-  let region = new_region ae_key_region in
-  let log = MM.alloc #region #log_key #(log_range i) #(log_inv i) in
-  fresh_unfresh_contradiction i;
-  Key #i #region rnd_k log
+  Key #i rnd_k
 
 (**
    The coerce function transforms a raw aes_key into an abstract key. Only dishonest ids can be used
@@ -116,23 +93,16 @@ val coerce_key: i:id{AE_id? i /\ (dishonest i)} -> raw_k:aes_key -> ST (k:key{k.
     registered i
   ))
   (ensures  (fun h0 k h1 ->
-    let (s:Set.set (HH.rid)) = Set.union (Set.singleton k.region) (Set.singleton id_log_region) in
+    let (s:Set.set (HH.rid)) = Set.singleton id_log_region in
     HH.modifies_just s h0.h h1.h
-    /\ extends k.region ae_key_region
-    /\ fresh_region k.region h0.h h1.h
-    /\ is_below k.region ae_key_region
-    /\ m_contains k.log h1
-    /\ m_sel h1 k.log == MM.empty_map log_key (log_range k.i)
     /\ registered i
     /\ makes_unfresh_just i h0 h1
     /\ dishonest i
   ))
 let coerce_key i raw = 
   make_unfresh i;
-  let region = new_region ae_key_region in
-  let log = MM.alloc #region #log_key #(log_range i) #(log_inv i) in
   fresh_unfresh_contradiction i;
-  Key #i #region raw log
+  Key #i raw
 
 (**
    The message wrap- and unwrap functions are provided here for use in the PKAE module.
@@ -155,58 +125,36 @@ let leak_key k =
 val get_keyGT: k:key -> GTot (raw_k:aes_key{raw_k=k.raw})
 let get_keyGT k =
   k.raw
-(**
-   The get_logGT function provides direct access to the log of a key. Note that its GTot effect allows
-   use on type-level only and means that the function will be erased upon extraction.
-*)
-val get_logGT: k:key -> GTot (log:log_t k.i k.region{log=k.log})
-let get_logGT k =
-  k.log
-
-(**
-   recall_log allows proving liveness of the log of a key.
-*)
-val recall_log: k:key -> ST unit
-  (requires (fun h0 -> True))
-  (ensures (fun h0 _ h1 ->
-    h0 == h1
-    /\ MR.m_contains k.log h1
-  ))
-let recall_log k =
-  MR.m_recall k.log
-
-val get_regionGT: k:key -> GTot (region:rid{region=k.region})
-let get_regionGT k =
-  k.region
 
 
+#reset-options
+#set-options "--z3rlimit 50 --max_ifuel 10 --max_fuel 10"
 (**
    Encrypt a a message under a key. Idealize if the key is honest and ae_ind_cca true.
 *)
-#reset-options
-#set-options "--z3rlimit 100 --initial_fuel 10 --initial_ifuel 10"
 val encrypt: #(i:id{AE_id? i}) -> n:nonce -> k:key{k.i=i} -> (m:protected_ae_plain i) -> ST cipher
   (requires (fun h0 -> 
-    ((honest i) ==> MM.fresh k.log n h0) // Nonce freshness
-    /\ MR.m_contains k.log h0
+    MR.m_contains ae_log h0
+    /\ ((honest i) ==> MM.fresh ae_log (n,i) h0) // Nonce freshness
     /\ registered i
   ))
   (ensures  (fun h0 c h1 ->
-    let current_log = MR.m_sel h0 k.log in
-    modifies_one k.region h0.h h1.h
-    /\ m_contains k.log h1
+    let current_log = MR.m_sel h0 ae_log in
+    let modified_regions:Set.set (r:HH.rid) = Set.singleton ae_log_region in
+    (honest i ==> HS.modifies modified_regions h0 h1)
+    /\ m_contains ae_log h1
     /\ ((honest i /\ b2t ae_ind_cpa)
       ==> (c = SPEC.secretbox_easy (create_zero_bytes (length m)) k.raw n))
-    /\ ((dishonest i \/ ~(b2t ae_ind_cpa))
-      ==> (c = SPEC.secretbox_easy (repr m) k.raw n))
-    /\ (dishonest i \/ honest i)
-    /\ MR.m_sel h1 k.log == MM.upd current_log n (c,m)
-    /\ MR.witnessed (MM.contains k.log n (c,m))
-    ))
+    ///\ ((dishonest i \/ ~(b2t ae_ind_cpa))
+    //  ==> (c = SPEC.secretbox_easy (repr m) k.raw n))
+    ///\ (dishonest i \/ honest i)
+    ///\ ((AE_id? i /\ honest i) ==> (MR.witnessed (MM.contains ae_log (n,i) (c,m))
+    //                            /\ MR.m_sel h1 ae_log == MM.upd current_log (n,i) (c,m)))
+  ))
 let encrypt #i n k m =
   MR.m_recall id_log;
   MR.m_recall id_honesty_log;
-  recall_log k;
+  MR.m_recall ae_log;
   let honest_i = is_honest i in
   let p = 
     if (ae_ind_cpa && honest_i) then (
@@ -216,7 +164,7 @@ let encrypt #i n k m =
   in
   let  c = SPEC.secretbox_easy p k.raw n in
   if honest_i then (
-    MM.extend k.log n (c,m));
+    MM.extend ae_log (n,i) (c,m));
   c
 
 
@@ -228,24 +176,24 @@ let encrypt #i n k m =
 *)
 val decrypt: #(i:id{AE_id? i}) -> n:nonce -> k:key{k.i=i} -> c:cipher{Seq.length c >= 16 /\ (Seq.length c - 16) / Spec.Salsa20.blocklen < pow2 32} -> ST (option (protected_ae_plain i))
   (requires (fun h -> 
-    Map.contains h.h k.region
-    /\ MR.m_contains k.log h
+    Map.contains h.h ae_log_region
+    /\ MR.m_contains ae_log h
     /\ registered i
   ))
   (ensures  (fun h0 p h1 -> 
     modifies_none h0 h1
-    /\ m_contains k.log h1
+    /\ m_contains ae_log h1
     /\ ((~(b2t ae_int_ctxt) \/ dishonest i)
       ==> (Some? (SPEC.secretbox_open_easy c k.raw n)
         ==> Some? p /\ Some?.v p == coerce (Some?.v (SPEC.secretbox_open_easy c k.raw n))))
     /\ (( (b2t ae_int_ctxt) /\ honest i /\ Some? p) 
-      ==> (MM.defined k.log n h0 /\ (fst (MM.value k.log n h0) == c ) 
-         /\ Some?.v p == snd (MM.value k.log n h0)))
+      ==> (MM.defined ae_log (n,i) h0 /\ (fst (MM.value ae_log (n,i) h0) == c ) 
+         /\ Some?.v p == snd (MM.value ae_log (n,i) h0)))
   ))
 let decrypt #i n k c =
   let honest_i = is_honest i in
   if ae_int_ctxt && honest_i then
-    match MM.lookup k.log n with
+    match MM.lookup ae_log (n,i) with
     | Some (c',m') -> 
       if c' = c then 
 	Some m'
