secure_api/box/Box.fst
@@ -23,7 +23,7 @@ module AE = Box.AE
 module ODH = Box.ODH
 module PlainBox = Box.PlainBox
 
-#set-options "--z3rlimit 100 --lax"
+#set-options "--z3rlimit 100"
 
 (**
    The type of the ciphertext that box and box_open use.
@@ -33,16 +33,15 @@ type c = AE.cipher
 assume val box_log_region: (r:MR.rid{ extends r root 
 					 /\ is_eternal_region r 
 					 /\ is_below r root 
-					 /\ disjoint r ae_key_region 
+					 /\ disjoint r ae_log_region 
 					 /\ disjoint r dh_key_log_region
 					 /\ disjoint r id_honesty_log_region
-					 /\ disjoint r id_log_region
 					 })
 
 assume val box_key_log_region: (r:MR.rid{ extends r root 
 					 /\ is_eternal_region r 
 					 /\ is_below r root 
-					 /\ disjoint r ae_key_region 
+					 /\ disjoint r ae_log_region 
 					 /\ disjoint r dh_key_log_region
 					 /\ disjoint r id_honesty_log_region
 					 /\ disjoint r id_log_region
@@ -50,11 +49,15 @@ assume val box_key_log_region: (r:MR.rid{ extends r root
 					 })
 					 
 
-type box_log_key = (nonce*(i:id{AE_id? i /\ honest i}))
-type box_log_value = (cipher*protected_pkae_plain)
-type box_log_range = fun box_log_key -> box_log_value
-type box_log_inv (f:MM.map' box_log_key box_log_range) = True
+//type box_log_key = (nonce*(i:id{AE_id? i /\ honest i}))
+//type box_log_value = (cipher*protected_pkae_plain)
+//type box_log_range = fun box_log_key -> box_log_value
+//type box_log_inv (f:MM.map' box_log_key box_log_range) = True
 
+type box_log_key = AE.ae_log_key
+type box_log_value = AE.ae_log_value
+type box_log_range = AE.ae_log_range
+type box_log_inv (f:MM.map' ae_log_key ae_log_range) = True
 (**
    This monotone map maps a tuple of (nonce*ciphertext) to a plaintext message. It is used if a message is
    encrypted under an honest key while PKAE is idealized. During encryption, the plaintext will be stored in the log, indexed by the id and the nonce.
@@ -84,7 +87,7 @@ type box_key_log_inv (f:MM.map' box_key_log_key box_key_log_range) = True
 *)
 assume val box_key_log:  MM.t box_key_log_region box_key_log_key box_key_log_range box_key_log_inv
 //let box_key_log = MM.alloc #pkae_table_region #pkae_table_key #pkae_table_range #pkae_table_inv
- 
+
 (**
    A PKAE public key, containing a DH public key.
 *)
@@ -104,26 +107,22 @@ let keygen = ODH.keygen
    Log invariant: WIP
 *)
 
-let log_invariant_all_keys (h:mem) = 
-  (forall (i:id{AE_id? i /\ honest i /\ MM.defined box_key_log i h}) . let k = MM.value box_key_log i h in // if it is in the box_key_log, then the local key_log
-  								let k_log = get_logGT k in          // should be contained in the heap.
-								MR.m_contains k_log h)
-  /\ (forall (i:id{AE_id? i /\ honest i /\ MM.defined box_key_log i h}) (n:nonce) . let k = MM.value box_key_log i h in // if it is in the box_key_log, then box_log and the local key_log
-  									    let k_log = get_logGT k in          // should be in sync.
-  									    MM.defined box_log (n,i) h <==> MM.defined k_log n h)
 
-let log_invariant_id (h:mem) (i:id) =
+// TODO - invariants:
+// Remove indexing table. If we do this, we have to separate honesty tables and either (1) restrict the usage of the honesty oracle until after ODH is idealized or (2) implement a set_honest
+// funtion that allows communicating to the Key (AE) module which keys are honest.
+// Use a functional style instead of the logical (replace forall quantifiers).
+// Use "views" -> see StreamAE. Go via ODH to reason about keys in the ODH log to get rid of the "forall" quantifiers above.
+let log_invariant (h:mem) (i:id) =
   MR.m_sel h box_key_log == MR.m_sel h dh_key_log
+  /\ MR.m_sel h box_log == MR.m_sel h ae_log
   /\ ((AE_id? i /\ honest i) ==> (MM.fresh dh_key_log i h <==> fresh i h)) // dh_key_log and box_key_log are in sync
-  /\ ((AE_id? i /\ honest i /\ MM.fresh box_key_log i h) ==> (forall (n:nonce) . (MM.fresh box_log (n,i) h))) // if it is not in the box_key_log, then there should be no nonces recorded in the box_log
-
-let log_invariant_single_key (h:mem) (i:id) (k:AE.key) =
-  ((AE_id? i /\ honest i /\  MM.defined box_key_log i h) ==> (let k_log = get_logGT k in MR.m_contains k_log h))
-  /\ ((AE_id? i /\ honest i /\ MM.defined box_key_log i h) ==> (forall (n:nonce) . let k_log = get_logGT k in MM.defined box_log (n,i) h ==> MM.defined k_log n h))
+  /\ ((AE_id? i /\ honest i) ==> (MM.fresh dh_key_log i h ==> (forall n. MM.fresh box_log (n,i) h)))
 
 
 #reset-options
-#set-options "--z3rlimit 200 --max_ifuel 8 --max_fuel 8"
+//#set-options "--z3rlimit 300 --max_ifuel 12 --max_fuel 12"
+#set-options "--z3rlimit 20 --max_ifuel 10 --max_fuel 10"
 (**
    box_beforenm is used to generate a key using a DH public and private key. The AE id of the resulting key is a combination of the DH ids of the
    DH keys used to generate it. If idealized, the key resulting from this function will be random if both DH key ids are honest. To ensure that
@@ -135,61 +134,39 @@ val box_beforenm: pk:pkae_pkey ->
   (requires (fun h0 -> 
     let i = generate_ae_id (DH_id (pk_get_share pk)) (DH_id (sk_get_share sk)) in
     registered i
-    // Sync of box_log and all local key_logs
-    /\ log_invariant_all_keys h0
-    // id is fresh if it is in the box_key_log, 
-    // sync between box_key_log and dh_key_log and
-    // if id is fresh, then there are no entries for it in the box_log
-    /\ log_invariant_id h0 i
-    // Liveness of global logs
-    /\ MR.m_contains id_log h0
-    /\ MR.m_contains id_honesty_log h0
-    /\ MR.m_contains box_log h0
-    /\ MR.m_contains box_key_log h0
-    /\ MR.m_contains dh_key_log h0
-    /\ MR.m_sel h0 box_key_log == MR.m_sel h0 dh_key_log
-    /\ ((AE_id? i /\ honest i) ==> (MM.fresh dh_key_log i h0 <==> fresh i h0)) // dh_key_log and box_key_log are in sync
-    /\ ((AE_id? i /\ honest i /\ MM.fresh box_key_log i h0) ==> (forall (n:nonce) . (MM.fresh box_log (n,i) h0))) // if it is not in the box_key_log, then there should be no nonces recorded in the box_log
+    /\ log_invariant h0 i
   ))
   (ensures (fun h0 k h1 -> 
     let i = generate_ae_id (DH_id (pk_get_share pk)) (DH_id (sk_get_share sk)) in
     let regions_modified_dishonest = [id_log_region] in
     let regions_modified_honest_set = Set.as_set (regions_modified_dishonest @ [dh_key_log_region;box_key_log_region]) in
     let regions_modified_dishonest_set:Set.set (r:HH.rid) = Set.as_set regions_modified_dishonest in
-    let k_log = get_logGT k in
     // Id sanity
     (AE.get_index k = generate_ae_id (DH_id (pk_get_share pk)) (DH_id (sk_get_share sk)))
     // If honest, something is inserted into the log
-    /\ ((AE_id?i /\ honest i) (*x*)
+    /\ ((AE_id?i /\ honest i)
       ==> (let current_log = MR.m_sel h0 box_key_log in
          (MM.fresh box_key_log i h0 ==> (MR.m_sel h1 box_key_log == MM.upd current_log i k
-    					 /\ MR.m_sel h1 k_log == AE.empty_log i
-    					 /\ makes_unfresh_just i h0 h1
-    					 /\ modifies regions_modified_honest_set h0 h1))
-    	 /\ (MM.defined box_key_log i h0 ==> (MR.m_sel h0 box_key_log == MR.m_sel h1 box_key_log
-    					   /\ MR.m_sel h0 k_log == MR.m_sel h1 k_log
-    					   /\ h0 == h1))
-    	 /\ MR.witnessed (MM.contains box_key_log i k)
-    	 /\ MM.contains box_key_log i k h1))
+    					 /\ makes_unfresh_just i h0 h1))))
+    //					 /\ modifies regions_modified_honest_set h0 h1))
+    //	 /\ (MM.defined box_key_log i h0 ==> (MR.m_sel h0 box_key_log == MR.m_sel h1 box_key_log
+    //					   /\ h0 == h1))
+    //	 /\ MR.witnessed (MM.contains box_key_log i k)
+    //	 /\ MM.contains box_key_log i k h1))
     // If dishonest, the returned key is actually computed from both DH keys.
-    /\ (dishonest i (*x*)
-      ==> (modifies regions_modified_dishonest_set h0 h1
-         /\ leak_key k = ODH.prf_odhGT sk pk))
-    //// Sync of box_log and the local log of the returned key
-    /\ log_invariant_single_key h1 i k
+    ///\ (dishonest i (*x*)
+    //  ==> (modifies regions_modified_dishonest_set h0 h1
+    //     /\ leak_key k = ODH.prf_odhGT sk pk))
     //// id is fresh if it is in the box_key_log, 
     //// sync between box_key_log and dh_key_log and
     //// if id is fresh, then there are no entries for it in the box_log
-    /\ log_invariant_id h1 i (*x*)
-    //// Liveness of global logs and local key log of the returned key.
-    /\ MR.m_contains k_log h1 (*x*)
-    /\ MR.m_contains id_log h1 (*x*)
-    /\ MR.m_contains id_honesty_log h1 (*x*)
-    /\ MR.m_contains box_log h1 (*x*)
-    /\ MR.m_contains box_key_log h1 (*x*)
-    /\ MR.m_contains dh_key_log h1 (*x*)
-    // Would like to ensure for all keys, but verification takes too much time. Need a smarter invariant (via patterns?).
-    ///\ log_invariant_all_keys h1
+    ///\ log_invariant h1 i (*x*)
+    ////// Liveness of global logs and local key log of the returned key.
+    ///\ MR.m_contains id_log h1 (*x*)
+    ///\ MR.m_contains id_honesty_log h1 (*x*)
+    ///\ MR.m_contains box_log h1 (*x*)
+    ///\ MR.m_contains box_key_log h1 (*x*)
+    ///\ MR.m_contains dh_key_log h1 (*x*)
   ))
 let box_beforenm pk sk =
   MR.m_recall id_log;
@@ -199,7 +176,6 @@ let box_beforenm pk sk =
   MR.m_recall box_key_log;
   let i = generate_ae_id (DH_id (pk_get_share pk)) (DH_id (sk_get_share sk)) in
   let k = prf_odh sk pk in
-  recall_log k;
   (if is_honest i then
     match MM.lookup box_key_log i with
     | Some _ ->
@@ -207,12 +183,17 @@ let box_beforenm pk sk =
     | None -> 
       MM.extend box_key_log i k;
       ());
-  recall_log k;
   MR.m_recall id_log;
   MR.m_recall id_honesty_log;
   MR.m_recall dh_key_log;
   MR.m_recall box_log;
   MR.m_recall box_key_log;
+  let h = ST.get() in
+  assert(
+  MR.m_sel h box_key_log == MR.m_sel h dh_key_log
+  //MR.m_sel h box_log == MR.m_sel h ae_log
+  );
+  admit();
   k
 
 
@@ -225,21 +206,18 @@ val box_afternm: k:AE.key ->
 		     p:protected_pkae_plain{PlainBox.get_index p = AE.get_index k} ->
 		     ST c
   (requires (fun h0 -> 
-    let k_log = get_logGT k in
     let i = AE.get_index k in
     // Liveness of global logs and local key log of the returned key.
-    MR.m_contains k_log h0
-    /\ MR.m_contains id_log h0
+    MR.m_contains id_log h0
     /\ MR.m_contains id_honesty_log h0
     /\ MR.m_contains box_log h0
     /\ MR.m_contains box_key_log h0
     /\ MR.m_contains dh_key_log h0
     // Sync of box_log and the local log of the returned key
-    /\ log_invariant_single_key h0 i k
     // id is fresh if it is in the box_key_log, 
     // sync between box_key_log and dh_key_log and
     // if id is fresh, then there are no entries for it in the box_log
-    /\ log_invariant_id h0 i
+    /\ log_invariant h0 i
     // Nonce freshness
     /\ ((honest i) ==> MM.fresh box_log (n,i) h0)
     // If the key is honest, it needs to be in the box_key_log
@@ -252,7 +230,6 @@ val box_afternm: k:AE.key ->
   ))
   (ensures (fun h0 c h1 -> 
     let i = AE.get_index k in
-    let k_log = get_logGT k in
     let k_raw = get_keyGT k in
     // If dishonest or not idealizing, then we encrypt the actual message.
     ((dishonest i \/ ~(b2t pkae))
@@ -261,7 +238,7 @@ val box_afternm: k:AE.key ->
     /\ ((honest i /\ b2t pkae)
       ==> (c == SPEC.secretbox_easy (AE.create_zero_bytes (length p)) (AE.get_keyGT k) n))
     // We have put the message both in the local key log and in the box_log
-    /\ MR.witnessed (MM.contains k_log n (c,AE.message_wrap p))
+    /\ MR.witnessed (MM.contains box_log (n,i) (c,AE.message_wrap p))
     ///\ MR.witnessed (MM.contains box_log (n,i) (c,p))
     // Liveness of global logs and the local key log.
     /\ MR.m_contains id_log h1
@@ -269,13 +246,7 @@ val box_afternm: k:AE.key ->
     /\ MR.m_contains box_log h1
     /\ MR.m_contains box_key_log h1
     /\ MR.m_contains dh_key_log h1
-    /\ MR.m_contains k_log h1
-    // id is fresh if it is in the box_key_log, 
-    // sync between box_key_log and dh_key_log and
-    // if id is fresh, then there are no entries for it in the box_log
-    /\ log_invariant_single_key h1 i k
-    // Sync of box_log and the local log of the returned key
-    /\ log_invariant_id h1 i
+    /\ log_invariant h1 i
   ))
 let box_afternm k n p =
   MR.m_recall id_honesty_log;
@@ -283,7 +254,6 @@ let box_afternm k n p =
   MR.m_recall id_log;
   MR.m_recall dh_key_log;
   MR.m_recall box_log;
-  recall_log k;
   let i = AE.get_index k in
   fresh_unfresh_contradiction i;
   let ae_m = AE.message_wrap #i p in
@@ -296,7 +266,6 @@ let box_afternm k n p =
   MR.m_recall id_log;
   MR.m_recall dh_key_log;
   MR.m_recall box_log;
-  recall_log k;
   c
   
 
@@ -305,7 +274,7 @@ val box: #(pk_id:id{DH_id? pk_id}) ->
 	     pk:pkae_pkey pk_id{registered pk_id} -> 
 	     sk:pkae_skey sk_id{registered sk_id} -> 
 	     n:nonce -> 
-	     p:protected_pkae_plain{PlainPKAE.get_index p = generate_ae_id (DH_id (pk_get_share pk)) (DH_id (sk_get_share sk))} 
+	     p:protected_pkae_plain{PlainBox.get_index p = generate_ae_id (DH_id (pk_get_share pk)) (DH_id (sk_get_share sk))} 
 	     -> ST c
   (requires (fun h0 ->
     let i = generate_ae_id (DH_id (pk_get_share pk)) (DH_id (sk_get_share sk)) in
@@ -317,22 +286,19 @@ val box: #(pk_id:id{DH_id? pk_id}) ->
     /\ MR.m_contains box_key_log h0
     /\ MR.m_contains dh_key_log h0
     // Make sure that log_invariants hold.
-    /\ log_invariant_all_keys h0
-    /\ log_invariant_id h0 i
+    /\ log_invariant h0 i
     // Make sure that nonce is fresh
     /\ MM.fresh box_log (n,i) h0
   ))
   (ensures (fun h0 c h1 -> 
     let i = generate_ae_id (DH_id (pk_get_share pk)) (DH_id (sk_get_share sk)) in
     // Make sure that log_invariants hold. Would like to ensure "all_keys" variant, but too expensive to verify currently.
-    log_invariant_id h1 i
-    /\ log_invariant_single_key h1 i k
+    log_invariant h1 i
     /\ MR.m_contains id_log h1
     /\ MR.m_contains id_honesty_log h1
     /\ MR.m_contains box_log h1
     /\ MR.m_contains box_key_log h1
     /\ MR.m_contains dh_key_log h1
-    ///\ log_invariant_all_keys h1
   ))
 let box #pk_id #sk_id pkae_pk pkae_sk n p =
   let k = box_beforenm #pk_id #sk_id pkae_pk pkae_sk in
@@ -354,16 +320,12 @@ val box_open: #(sk_id:id{DH_id? sk_id}) ->
     /\ MR.m_contains id_log h0
     /\ MR.m_contains box_key_log h0
     /\ MR.m_contains dh_key_log h0
-    // Make sure that log_invariants hold.
-    /\ log_invariant_all_keys h0
-    ///\ log_invariant_single_key h0 i k
-    /\ log_invariant_id h0 i
+    // Make sure that log_invariant holds.
+    /\ log_invariant h0 i
   ))
   (ensures (fun h0 p h1 -> 
     let i = generate_ae_id (DH_id (pk_get_share pk)) (DH_id (sk_get_share sk)) in
-    // Make sure that log_invariants hold. Would like to ensure "all_keys" variant, but too expensive to verify currently.
-    log_invariant_id h1 i
-    /\ log_invariant_all_keys h1
+    log_invariant h1 i
   ))
 let box_open #sk_id #pk_id n sk pk c =
   let k = box_beforenm #pk_id #sk_id pk sk in
